Update Compile.v to accommodate changes
Incorporate changes made previously to Compile.v and adapt them to
accommodate changes made elsewhere in fiat2 (specifically in Language.v
and Interpret.v).

fiat2/src/fiat2/Compile.v
@@ -102,7 +102,6 @@ Section WithMap.
           {tenv : map.map string (type * bool)} {tenv_ok : map.ok tenv}
           {locals : map.map string {t & interp_type (word := word) t}} {locals_ok : map.ok locals}
           {locals' : map.map string word} {locals'_ok : map.ok locals'}
-          {env : map.map String.string (list String.string * list String.string * Syntax.cmd)}
           {ext_spec : ExtSpec}.
 
   (* Relation between source language and target language values,
@@ -181,46 +180,56 @@ Section WithMap.
       assumption.
   Qed.
 
-  Definition tenv_relation (G : tenv) (lo : locals) : Prop :=
+  Definition tenv_relation (G : tenv) (store env : locals) : Prop :=
     map.forall_keys (fun key =>
     match map.get G key with
-    | Some (t, _) => match map.get lo key with
-                     | Some (existT _ t' _) => t = t'
-                     | None => False
-                     end
+    | Some (t, false) => match map.get env key with
+                         | Some (existT _ t' _) => t = t'
+                         | None => False
+                         end
+    | Some (t, true) => match map.get store key with
+                        | Some (existT _ t' _) => t = t'
+                        | None => False
+                        end
     | None => True
     end) G.
 
-  Lemma tenv_relation_get (G : tenv) (lo : locals) :
-    tenv_relation G lo -> forall (x : string) (t : type) (b : bool),
+  Lemma tenv_relation_get (G : tenv) (store env : locals) :
+    tenv_relation G store env -> forall (x : string) (t : type) (b : bool),
     map.get G x = Some (t, b) -> exists (v : interp_type t),
-    map.get lo x = Some (existT _ t v).
+    map.get (if b then store else env) x = Some (existT _ t v).
   Proof.
     intros Hlo x t b Htb.
     unfold tenv_relation, map.forall_keys in Hlo.
     specialize Hlo with (1 := Htb).
     rewrite Htb in Hlo.
-    destruct map.get.
-    - destruct s. subst. now exists i.
-    - destruct Hlo.
+    destruct b.
+    all: destruct map.get;
+    [ destruct s; subst; now exists i
+    | destruct Hlo ].
   Qed.
 
-  Lemma tenv_relation_put (G : tenv) (lo : locals) :
-    tenv_relation G lo ->
+  Lemma tenv_relation_put (G : tenv) (store env : locals) :
+    tenv_relation G store env ->
     forall (x : string) (t : type) (b : bool) (v : interp_type t),
-    tenv_relation (map.put G x (t, b)) (set_local lo x v).
+    if b then
+    tenv_relation (map.put G x (t, b)) (set_local store x v) env
+    else
+    tenv_relation (map.put G x (t, b)) store (set_local env x v).
   Proof.
     intros Hlo x t b v.
     unfold tenv_relation, map.forall_keys, set_local.
-    intros x' [t' b'].
-    repeat rewrite Properties.map.get_put_dec.
-    destruct (x =? x')%string.
-    - easy.
-    - intros Hx'. fwd.
-      unfold tenv_relation, map.forall_keys in Hlo.
-      specialize Hlo with (1 := Hx').
-      rewrite Hx' in Hlo.
-      assumption.
+    destruct b.
+    all:
+    intros x' [t' b'];
+    repeat rewrite Properties.map.get_put_dec;
+    destruct (x =? x')%string;
+    [ easy
+    | intros Hx'; fwd;
+      unfold tenv_relation, map.forall_keys in Hlo;
+      specialize Hlo with (1 := Hx');
+      rewrite Hx' in Hlo;
+      assumption ].
   Qed.
 
   Lemma proj_expected_existT (t : type) (v : interp_type t) :
@@ -234,11 +243,10 @@ Section WithMap.
     trivial.
   Qed.
 
-  (*
-  Lemma interp_type_eq : forall {t : type} (e : expr t) (w : interp_type t) (l : locals),
+  Lemma interp_type_eq : forall {t : type} (e : expr t) (w : interp_type t) (store env : locals),
     (existT interp_type t w =
-    existT interp_type t (interp_expr l e)) ->
-    (interp_expr l e) = w.
+    existT interp_type t (interp_expr store env e)) ->
+    (interp_expr store env e) = w.
   Proof.
     intros.
     inversion_sigma.
@@ -246,7 +254,6 @@ Section WithMap.
     * easy.
     * exact type_eq_dec.
   Qed.
-  *)
 
   Lemma eval_map_extends_locals : forall e (m : mem) (l l' : locals') w,
     map.extends l' l ->
@@ -292,111 +299,144 @@ Section WithMap.
         now rewrite H2.
   Qed.
 
-  (*
   Lemma compile_correct :
     forall {t} (e : expr t) (e' : Syntax.expr) (G : tenv),
     wf G e ->
-    compile_expr e = Success e' -> forall lo l,
-    tenv_relation G lo ->
-    locals_relation lo l -> exists w : word, forall m,
+    compile_expr e = Success e' -> forall store env l,
+    tenv_relation G store env ->
+    locals_relation store l -> locals_relation env l ->
+    exists w : word, forall m,
     eval_expr m l e' = Some w /\
-    value_relation (interp_expr lo e) w.
-    (* forall tr m l, *)
-    (* exec map.empty c tr m l (fun tr' m' l' => exists (w : word), *)
-    (*   eval_expr m' l' e' = Some w /\ *)
-    (*   value_relation (interp_expr map.empty map.empty e) w /\ *)
-    (*   m' = m /\ *)
-    (*   map.extends l' l *)
-    (* ). *)
+    value_relation (interp_expr store env e) w.
   Proof.
-    intros t. induction e; intros c e' He He' tr m l; try easy.
+    intros t. induction e; intros e' G He He' store env l HG Hstore Henv; try easy.
+    - (* EVar x *)
+      unfold compile_expr in He'.
+      fwd.
+      simpl.
+      inversion_clear He.
+      edestruct tenv_relation_get as [v Hv].
+      { exact HG. }
+      { exact H. }
+      simpl in Hv.
+      edestruct locals_relation_get as [w Hw].
+      { exact Henv. }
+      { exact t. }
+      { exact Hv. }
+      exists w.
+      intros _; split.
+      { assumption. }
+      unfold get_local.
+      rewrite Hv.
+      unfold locals_relation, map.forall_keys in Henv.
+      specialize Henv with (1 := Hv).
+      rewrite Hv, Hw in Henv.
+      now rewrite <- proj_expected_existT.
+    - (* ELoc x *)
+      unfold compile_expr in He'.
+      fwd.
+      simpl.
+      inversion_clear He.
+      edestruct tenv_relation_get as [v Hv].
+      { exact HG. }
+      { exact H. }
+      simpl in Hv.
+      edestruct locals_relation_get as [w Hw].
+      { exact Hstore. }
+      { exact t. }
+      { exact Hv. }
+      exists w.
+      intros _; split.
+      { assumption. }
+      unfold get_local.
+      rewrite Hv.
+      unfold locals_relation, map.forall_keys in Hstore.
+      specialize Hstore with (1 := Hv).
+      rewrite Hv, Hw in Hstore.
+      now rewrite <- proj_expected_existT.
     - (* EAtom a *)
       unfold compile_expr in He'.
       fwd.
-      apply exec.skip.
+      simpl.
       destruct a; try easy.
-      + (* AInt n *)
-        injection E as [= <-].
+      + (* AWord n *)
         simpl.
+        simpl in He'.
+        fwd.
         exists (word.of_Z (word.wrap n)).
-        ssplit; try easy;
+        intros m; split;
         rewrite <- word.unsigned_of_Z, word.of_Z_unsigned; try easy.
         apply RWord.
       + (* ABool b *)
-        injection E as [= <-].
         simpl.
+        simpl in He'.
+        fwd.
         exists (word.of_Z (Z.b2z b)).
-        ssplit; try easy.
+        intros m; split; try easy.
         apply RBool.
     - (* EUnop o e *)
       destruct o; try easy.
       all:
-        simpl in He';
         simpl;
-        fwd;
+        simpl in He';
+        fwd; rename a into e', E into He';
         inversion He;
-        apply Eqdep_dec.inj_pair2_eq_dec in H4 as [= ->]; try exact type_eq_dec;
-        specialize IHe with (2 := eq_refl);
-        eapply exec.weaken; [ now apply IHe |];
-        cbv beta;
-        intros tr' m' l' Hw;
+        apply Eqdep_dec.inj_pair2_eq_dec in H3, H4 as [= ->]; try exact type_eq_dec;
+        apply Eqdep_dec.inj_pair2_eq_dec in H3 as [= ->]; try exact type_eq_dec;
+        subst;
+        specialize IHe with (1 := H2) (2 := eq_refl) (3 := HG) (4 := Hstore) (5 := Henv);
         fwd;
         eexists;
-        ssplit;
-        [ simpl; now fwd
-        |
-        | reflexivity
-        | assumption ];
-        inversion Hwp1;
+        intros m; specialize IHe with m; fwd;
+        simpl;
+        rewrite IHep0;
+        split;
+        [ reflexivity |];
+        inversion IHep1;
         subst;
-        repeat lazymatch goal with
+        repeat (repeat lazymatch goal with
         | h: existT _ _ _ = existT _ _ _ |- _ =>
             apply interp_type_eq in h
         end;
-        subst.
+        subst).
       + (* OWNeg *)
         rewrite Properties.word.sub_0_l.
         apply RWord.
       + (* ONot *)
         rewrite <- Properties.word.ring_morph_sub.
-        destruct (interp_expr map.empty map.empty e); apply RBool.
+        destruct (interp_expr _ _ e); apply RBool.
     - (* EBinop o e1 e2 *)
       destruct o; try easy.
       all:
-        simpl in He';
         simpl;
-        fwd;
+        simpl in He';
+        fwd; rename a into e1', E into He1', a0 into e2', E0 into He2';
         inversion He;
-        apply Eqdep_dec.inj_pair2_eq_dec in H5 as [= ->]; try exact type_eq_dec;
-        injection H6 as [= ->];
-        apply Eqdep_dec.inj_pair2_eq_dec in H5 as [= ->]; try exact type_eq_dec;
-        specialize IHe1 with (2 := eq_refl);
-        specialize IHe2 with (2 := eq_refl);
-        eapply exec.seq; [ now apply IHe1 |];
-        cbv beta;
-        intros tr' m' l' Hw;
-        fwd;
-        eapply exec.weaken; [ now apply IHe2 |];
-        cbv beta;
-        intros tr'' m'' l'' Hw';
-        fwd;
-        eexists;
-        ssplit;
-        [ simpl; fwd;
-          apply eval_map_extends_locals with (l' := l'') in Hwp0;
-          [| assumption];
-          now rewrite Hwp0
-        |
-        | reflexivity
-        | now apply extends_trans with l' ].
-      1-9:
-        inversion Hwp1; inversion Hw'p1;
-        subst;
-        repeat lazymatch goal with
+        repeat (repeat lazymatch goal with
         | h: existT _ _ _ = existT _ _ _ |- _ =>
             apply interp_type_eq in h
         end;
+        subst);
+        apply Eqdep_dec.inj_pair2_eq_dec in H5, H6 as [= ->]; try exact type_eq_dec;
         subst;
+        specialize IHe1 with (1 := H3) (2 := eq_refl) (3 := HG) (4 := Hstore) (5 := Henv);
+        specialize IHe2 with (1 := H7) (2 := eq_refl) (3 := HG) (4 := Hstore) (5 := Henv);
+        fwd;
+        eexists;
+        intros m; specialize IHe1 with m; specialize IHe2 with m; fwd;
+        simpl;
+        rewrite IHe1p0, IHe2p0;
+        split;
+        [ reflexivity |].
+      1-9:
+        (* all except OEq *)
+        inversion IHe1p1; inversion IHe2p1;
+        subst;
+        repeat (repeat lazymatch goal with
+        | h: existT _ _ _ = existT _ _ _ |- _ =>
+            apply interp_type_eq in h
+        end;
+        subst);
         set (v1 := interp_expr _ _ e1);
         set (v2 := interp_expr _ _ e2).
       1-5:
@@ -422,24 +462,24 @@ Section WithMap.
       + (* OEq *)
         destruct t; try easy; unfold eqb_values.
         * (* TWord *)
-          inversion Hwp1; inversion Hw'p1.
-          repeat lazymatch goal with
-          | h: existT _ _ _ = existT _ _ _ |- _ =>
-              apply interp_type_eq in h
-          end.
-          subst.
-          destruct (word.eqb _ _);
-          apply RBool.
-        * (* TBool *)
-          inversion Hwp1; inversion Hw'p1.
-          repeat lazymatch goal with
+          inversion IHe1p1; inversion IHe2p1.
+          subst;
+          repeat (repeat lazymatch goal with
           | h: existT _ _ _ = existT _ _ _ |- _ =>
               apply interp_type_eq in h
           end;
-          subst.
-          set (b1 := interp_expr _ _ e1).
-          set (b2 := interp_expr _ _ e2).
-          destruct b1, b2.
+          subst).
+          destruct word.eqb;
+          apply RBool.
+        * (* TBool *)
+          inversion IHe1p1; inversion IHe2p1.
+          subst;
+          repeat (repeat lazymatch goal with
+          | h: existT _ _ _ = existT _ _ _ |- _ =>
+              apply interp_type_eq in h
+          end;
+          subst).
+          destruct (interp_expr _ _ e1) eqn:E1, (interp_expr _ _ e2) eqn:E2.
           all:
             apply RBool';
             simpl;
@@ -447,7 +487,6 @@ Section WithMap.
             try rewrite word.unsigned_of_Z_0;
             now try rewrite word.unsigned_of_Z_1.
   Qed.
-  *)
 
 End WithMap.
 
